src/Compilers/Z/Named/RewriteAddToAdcInterp.v
@@ -1,0 +1,1572 @@
+Require Import Coq.ZArith.ZArith.
+Require Import Crypto.Compilers.Named.Context.
+Require Import Crypto.Compilers.Named.ContextDefinitions.
+Require Import Crypto.Compilers.Named.ExprInversion.
+Require Import Crypto.Compilers.Syntax.
+Require Import Crypto.Compilers.Z.Syntax.
+Require Import Crypto.Compilers.Z.Named.RewriteAddToAdc.
+Require Import Crypto.Compilers.Named.Syntax.
+Require Import Crypto.Util.Notations.
+Require Import Crypto.Util.Option.
+Require Import Crypto.Util.Tactics.DestructHead.
+Require Import Crypto.Util.Tactics.BreakMatch.
+Require Import Crypto.Util.Prod.
+Require Import Crypto.Util.LetIn.
+
+Local Open Scope Z_scope.
+
+Section named.
+  Context {interp_base_type : base_type -> Type}
+          {interp_op : forall s d, op s d -> interp_flat_type interp_base_type s -> interp_flat_type interp_base_type d}
+          {Name : Type}
+          {InterpContext : Context Name interp_base_type}
+          {InterpContextOk : ContextOk InterpContext}
+          (Name_beq : Name -> Name -> bool)
+          (Name_bl : forall n1 n2, Name_beq n1 n2 = true -> n1 = n2)
+          (Name_lb : forall n1 n2, n1 = n2 -> Name_beq n1 n2 = true).
+
+  Local Notation exprf := (@exprf base_type op Name).
+  Local Notation expr := (@expr base_type op Name).
+  Local Notation do_rewrite := (@do_rewrite Name Name_beq).
+  Local Notation do_rewriteo := (@do_rewriteo Name Name_beq).
+  Local Notation rewrite_exprf := (@rewrite_exprf Name Name_beq).
+  Local Notation rewrite_exprf_prestep := (@rewrite_exprf_prestep Name).
+  Local Notation rewrite_expr := (@rewrite_expr Name Name_beq).
+
+  Local Ltac t_step :=
+    first [ progress simpl in *
+          | reflexivity
+          | congruence
+          | progress unfold option_map, LetIn.Let_In in *
+          | progress intros
+          | progress subst
+          | progress inversion_option
+          | progress destruct_head' unit
+          | progress destruct_head'_prod
+          | progress inversion_prod
+          | solve [ f_equal; eauto ]
+          | match goal with
+            | [ H : interpf (t:=?T) ?e = Some ?v, H' : interpf _ = Some ?v' |- _ ]
+              => assert (v = v' :> interp_flat_type _ T) by eauto; (subst v || (progress inversion_prod))
+            | [ IH : context[interpf ?e], H' : interpf (ctx:=?ctx') ?e = Some _ |- _ ]
+              => specialize (fun v1 v2 => IH ctx' v1 v2); rewrite H' in IH
+            | [ H : forall v1 v2, Some _ = Some v1 -> _ |- _ ]
+              => specialize (fun v2 => H _ v2 eq_refl)
+            | [ H : forall v, Some _ = Some v -> _ |- _ ]
+              => specialize (H _ eq_refl)
+            | [ H : ?x = interp_op _ _ _ _, H' : context[?x] |- _ ]
+              => progress rewrite H in H'
+            | [ H : ?x = (_,_)%core, H' : context[?x] |- _ ]
+              => progress rewrite H in H'
+            end ].
+  Local Ltac t_destruct_step :=
+    match goal with
+    | [ e : exprf ?t |- context[match ?t with _ => _ end] ]
+      => is_var t; destruct e
+    | [ e : exprf ?t, H : context[match ?t with _ => _ end] |- _ ]
+      => is_var t; destruct e
+    | [ e : op ?s ?d |- context[match ?s with _ => _ end] ]
+      => is_var s; is_var d; destruct e
+    | [ e : op ?s ?d |- context[match ?d with _ => _ end] ]
+      => is_var s; is_var d; destruct e
+    | [ e : op ?s ?d, H : context[match ?s with _ => _ end] |- _ ]
+      => is_var s; is_var d; destruct e
+    | [ e : op ?s ?d, H : context[match ?d with _ => _ end] |- _ ]
+      => is_var s; is_var d; destruct e
+    end.
+  Local Ltac t'_step :=
+    first [ break_innermost_match_step
+          | break_innermost_match_hyps_step ].
+  Local Ltac t_invert_step :=
+    progress invert_expr; break_innermost_match; try exact I; intros.
+
+  Local Notation retT e re :=
+    (forall (ctx : InterpContext)
+            v,
+        Named.interpf (interp_op:=interp_op) (ctx:=ctx) re = Some v
+        -> Named.interpf (interp_op:=interp_op) (ctx:=ctx) e = Some v)
+      (only parsing).
+  Local Notation tZ := (Tbase TZ).
+  Local Notation ADC bw c x y := (Op (@AddWithGetCarry bw TZ TZ TZ TZ TZ)
+                                     (Pair (Pair (t1:=tZ) c (t2:=tZ) x) (t2:=tZ) y)).
+  Local Notation ADD bw x y := (ADC bw (Op (OpConst 0) TT) x y).
+  Local Notation ADX x y := (Op (@Add TZ TZ TZ) (Pair (t1:=tZ) x (t2:=tZ) y)).
+  Lemma interpf_do_rewrite
+        {t} {e e' : exprf t}
+        (H : do_rewrite e = Some e')
+    : retT e e'.
+  Proof.
+    (*refine match e return retT (do_rewrite rewrite_exprf) e with
+           |           (nlet (a2, c1) : tZ * tZ := (ADD bw1 a b as ex0) in P0)
+             => _(*match rewrite_exprf _ P0 in Named.exprf _ _ _ t return exprf t -> exprf t with
+            |      (nlet (s , c2) : tZ * tZ := (ADD bw2 c0 (Var _ a2') as ex1) in P1)
+              => match P1 in Named.exprf _ _ _ t return exprf t -> exprf t with
+                 | (nlet c        : tZ      := (ADX (Var _ c1') (Var _ c2') as ex2) in P)
+                   => fun e
+                      => if (((bw1 =Z? bw2) && (a2 =n? a2') && (c1 =n? c1') && (c2 =n? c2'))
+                               && (is_const_or_var c0 && is_const_or_var a && is_const_or_var b)
+                               && negb (name_list_has_duplicate (a2::c1::s::c2::c::nil ++ get_namesf c0 ++ get_namesf a ++ get_namesf b)%list))
+                         then (nlet (a2, c1) : tZ * tZ := ex0 in
+                               nlet (s , c2) : tZ * tZ := ex1 in
+                               nlet c        : tZ      := ex2 in
+                               nlet (s, c)   : tZ * tZ := ADC bw1 c0 a b in
+                               P)
+                         else e
+                 | P1' => fun e => e
+                 end
+            | P0' => fun e => e
+            end (nlet (a2, c1) : tZ * tZ := rewrite_exprf _ ex0 in rewrite_exprf _ P0)*)
+       | _ => _
+           end%core%nexpr%bool.
+    solve [ repeat first [ t_step ] ].
+    solve [ repeat first [ t_step ] ].
+    solve [ repeat first [ t_step | t'_step ] ].
+    solve [ repeat first [ t_step | t'_step ] ].
+    solve [ repeat first [ t_step | t'_step ] ].
+    Focus 7.
+    { repeat first [ t_step | t'_step ].
+      Require Import AdmitAxiom.
+      revert H H0.
+      Set Printing All.
+      admit.
+      lazymatch goal with
+      | [ H : match ?e with _ => _ end = _ |- _ ] => destruct e eqn:?
+      end.
+      destruct (lookupb ctx n) eqn:?.
+
+    repeat first [ t_step | t'_step ]. }
+      eapply IH.
+      2:eassumption.
+      rewrite <- H.
+      match goal with
+      | [ H : interpf (t:=?T) _ = Some ?x, H' : interpf _ = Some ?y |- _ ]
+        => assert (x = y :> interp_flat_type _ T) by eauto
+      end.
+      Arguments interpf : clear implicits.
+
+
+      etransitivity.
+      eapply H0.
+      Focus 4.
+      {
+        t_step.
+        Set Printing All.
+        clear.
+        assert(forall (ctx : @ContextT base_type Name interp_base_type InterpContext)
+    (v1 v2 : @interp_flat_type base_type interp_base_type f0)
+    (_ : @eq (option (@interp_flat_type base_type interp_base_type f0))
+           (@interpf base_type interp_base_type op Name InterpContext interp_op
+              (@extendb base_type Name interp_base_type InterpContext
+                 (@extendb base_type Name interp_base_type InterpContext ctx i TZ
+                    (@fst (interp_base_type TZ) (interp_base_type TZ) tt)) i0 TZ
+                 (@snd (interp_base_type TZ) (interp_base_type TZ) tt)) f0 eC)
+           (@Some (@interp_flat_type base_type interp_base_type f0) v1))
+    (_ : @eq (option (@interp_flat_type base_type interp_base_type f0))
+           match
+             @interpf base_type interp_base_type op Name InterpContext interp_op ctx
+               (@Prod base_type (@Tbase base_type TZ) (@Tbase base_type TZ))
+               (rewrite_exprf (@Prod base_type (@Tbase base_type TZ) (@Tbase base_type TZ))
+                  (@TT base_type op Name))
+             return (option (@interp_flat_type base_type interp_base_type f0))
+           with
+           | Some xv =>
+               @interpf base_type interp_base_type op Name InterpContext interp_op
+                 (@extendb base_type Name interp_base_type InterpContext
+                    (@extendb base_type Name interp_base_type InterpContext ctx i TZ
+                       (@fst (interp_base_type TZ) (interp_base_type TZ) xv)) i0 TZ
+                    (@snd (interp_base_type TZ) (interp_base_type TZ) xv)) f0
+                 (rewrite_exprf f0 eC)
+           | None => @None (@interp_flat_type base_type interp_base_type f0)
+           end (@Some (@interp_flat_type base_type interp_base_type f0) v2)),
+  @eq (@interp_flat_type base_type interp_base_type f0) v1 v2).
+        simpl.
+        first [progress simpl in * ].
+          | reflexivity  ].
+          | congruence ].
+          | progress unfold option_map, LetIn.Let_In in *
+          | progress intros
+          | progress subst
+          | progress inversion_option
+          | progress destruct_head' unit
+          | progress destruct_head'_prod
+          | progress inversion_prod ].
+          | solve [ f_equal; eauto ]
+          | match goal with
+            | [ H : interpf ?e = Some ?v, H' : interpf (rewrite_exprf ?e') = Some ?v' |- _ ]
+              => assert (v = v') by eauto; subst v
+            | [ IH : context[interpf ?e], H' : interpf (ctx:=?ctx') ?e = Some _ |- _ ]
+              => specialize (fun v1 v2 => IH ctx' v1 v2); rewrite H' in IH
+            | [ H : forall v1 v2, Some _ = Some v1 -> _ |- _ ]
+              => specialize (fun v2 => H _ v2 eq_refl)
+            | [ H : forall v, Some _ = Some v -> _ |- _ ]
+              => specialize (H _ eq_refl)
+            | [ H : ?x = interp_op _ _ _ _, H' : context[?x] |- _ ]
+              => progress rewrite H in H'
+            | [ H : ?x = (_,_)%core, H' : context[?x] |- _ ]
+              => progress rewrite H in H'
+            end ].
+
+        t_step.
+      4:try solve [ repeat first [ t_step ] ].
+      2:try solve [ repeat first [ t_step ] ].
+                 |
+     *)
+    (*
+    match goal with
+    end.
+    lazymatch goal with
+
+    end.
+    eauto.
+        by (rewrite <- H'; eauto); (subst v || (progress inversion_prod))
+    end.
+    all:simpl; unfold option_map in *.
+    all:repeat (break_innermost_match; break_innermost_match_hyps;
+        repeat t_step).
+    Focus 2.
+
+      repeat t_step.
+      intros *;
+      let H := fresh in
+      lazymatch goal with
+      | [ |- context[do_rewrite ?e] ]
+        => destruct (do_rewrite e) eqn:H;
+             [ pose proof (interpf_do_rewrite H) | ]
+      end;
+        try solve [ clear H; repeat first [ t_step | t'_step ] ].
+    Focus 2.
+    clear H.
+    { repeat t_step.
+      break_match_hyps; repeat t_step.
+      specialize (IHe1 _ Heqo0).
+      specialize (fun v1 pf => H0 v1 _ pf eq_refl).
+      specialize (IHe2 v2).
+      repeat first [ t_step | t'_step ].
+      specialize (IHe2 _ Heqo0).
+      specialize (fun v1 pf => H0 v1 _ pf eq_refl).
+      break_match_hyps; repeat t_step.
+      repeat first [ t_step | t'_step ].
+      [ repeat first [ t_step | t'_step ]
+      |
+      | repeat first [ t_step | t'_step ] ];
+      [].
+    intros.
+    break_innermost_match_hyps_step.
+    2:solve [ repeat first [ t_step | t'_step ] ].
+    all:break_innermost_match_hyps_step.
+    solve [ repeat first [ t_step | t'_step ] ].
+    solve [ repeat first [ t_step | t'_step ] ].
+    2:solve [ repeat first [ t_step | t'_step ] ].
+    2:solve [ repeat first [ t_step | t'_step ] ].
+    match goal with
+    | [ H : match ?e with _ => _ end = _ |- _ ] => destruct e eqn:?
+    end.
+    2:solve [ repeat first [ t_step | t'_step ] ].
+    unfold Let_In in *.
+    break_innermost_match_hyps_step.
+    2:solve [ repeat first [ t_step | t'_step ] ].
+    break_innermost_match_hyps_step.
+    2:solve [ repeat first [ t_step | t'_step ] ].
+    2:solve [ repeat first [ t_step | t'_step ] ].
+    break_innermost_match_hyps_step.
+    2:solve [ repeat first [ t_step | t'_step ] ].
+    break_innermost_match_hyps_step.
+    revert dependent e1; intro e1.
+    refine match e1 with
+           | TT => _
+           | _ => _
+           end.
+    solve [ repeat first [ t_step | t'_step ] ].
+    solve [ repeat first [ t_step | t'_step ] ].
+    break_innermost_match_step.
+    solve [ repeat first [ t_step | t'_step ] ].
+    solve [ repeat first [ t_step | t'_step ] ].
+    break_innermost_match_step.
+    break_innermost_match_step.
+    break_innermost_match_step.
+    break_innermost_match_step.
+    intros.
+    all:repeat match goal with
+           | [ H : context[match ?e with _ => _ end] |- _ = _ ]
+             => first [ is_var e; destruct e
+                      | revert dependent e ]
+           | [ |- context[match ?e with _ => _ end] ]
+             => first [ is_var e; destruct e
+                      | revert dependent e ]
+           | _ => exact I
+           | [ |- forall a : op ?s tZ, @?P a ]
+             => is_var s; intro a; move a at top; generalize dependent s;
+                  lazymatch goal with
+                  | [ |- forall s (a : op s tZ), @?P s a ]
+                    => intros s a;
+                         refine match a as a' in op s' d'
+                                      return match d' return op s' d' -> _ with
+                                             | tZ => fun a'' => P _ a''
+                                             | _ => fun _ => True
+                                             end a'
+                                with
+                                | OpConst _ _ => _
+                                | _ => _
+                                end;
+                         clear a;
+                         try exact I;
+                         intros
+                  end
+           | [ |- forall a : op ?s (tZ * tZ), @?P a ]
+             => is_var s; intro a; move a at top; generalize dependent s;
+                  lazymatch goal with
+                  | [ |- forall s (a : op s (tZ * tZ)), @?P s a ]
+                    => intros s a;
+                         refine match a as a' in op s' d'
+                                      return match d' return op s' d' -> _ with
+                                             | Prod tZ tZ => fun a'' => P _ a''
+                                             | _ => fun _ => True
+                                             end a'
+                                with
+                                | OpConst _ _ => _
+                                | _ => _
+                                end;
+                         clear a;
+                         try exact I;
+                         intros
+                  end
+           | [ |- forall e : exprf Unit, @?P e ]
+             => intro e;
+                  refine match e as e' in Named.exprf _ _ _ t
+                               return match t return exprf t -> _ with
+                                      | Unit => fun e' => P e'
+                                      | _ => fun _ => True
+                                      end e'
+                         with
+                         | TT => _
+                         | _ => _
+                         end;
+                  clear e;
+                  try exact I;
+                  intros
+           | [ |- forall e : exprf tZ, @?P e ]
+             => intro e;
+                  refine match e as e' in Named.exprf _ _ _ t
+                               return match t return exprf t -> _ with
+                                      | tZ => fun e' => P e'
+                                      | _ => fun _ => True
+                                      end e'
+                         with
+                         | TT => _
+                         | _ => _
+                         end;
+                  clear e;
+                  try exact I;
+                  intros
+           | [ |- forall e : exprf (tZ * tZ), @?P e ]
+             => intro e;
+                  refine match e as e' in Named.exprf _ _ _ t
+                               return match t return exprf t -> _ with
+                                      | (tZ * tZ)%ctype => fun e' => P e'
+                                      | _ => fun _ => True
+                                      end e'
+                         with
+                         | TT => _
+                         | _ => _
+                         end;
+                  clear e;
+                  try exact I;
+                  intros
+           | [ |- forall e : exprf (tZ * tZ * tZ), @?P e ]
+             => intro e;
+                  refine match e as e' in Named.exprf _ _ _ t
+                               return match t return exprf t -> _ with
+                                      | (tZ * tZ * tZ)%ctype => fun e' => P e'
+                                      | _ => fun _ => True
+                                      end e'
+                         with
+                         | TT => _
+                         | _ => _
+                         end;
+                  clear e;
+                  try exact I;
+                  intros
+           end.
+    solve [ repeat first [ t_step | t'_step ] ].
+    solve [ repeat first [ t_step | t'_step ] ].
+    solve [ repeat first [ t_step | t'_step ] ].
+    solve [ repeat first [ t_step | t'_step ] ].
+    solve [ repeat first [ t_step | t'_step ] ].
+    { match goal with
+           | [ H : context[match ?e with _ => _ end] |- _ = _ ]
+             => (tryif is_var e
+                  then fail
+                  else let e' := fresh in
+                       set (e' := e) in *;
+                       assert (e' = e) by reflexivity;
+                       clearbody e';
+                       first [ destruct e'
+                             | revert dependent e' ])
+    end.
+    solve [ repeat first [ t_step | t'_step ] ].
+    solve [ repeat first [ t_step | t'_step ] ].
+    solve [ repeat first [ t_step | t'_step ] ].
+    2:solve [ repeat first [ t_step | t'_step ] ].
+     match goal with
+           | [ H : context[match ?e with _ => _ end] |- _ = _ ]
+             => first [ is_var e; destruct e
+                      | revert dependent e ]
+           | [ |- context[match ?e with _ => _ end] ]
+             => first [ is_var e; destruct e
+                      | revert dependent e ]
+           | _ => exact I
+           | [ |- forall a : op ?s tZ, @?P a ]
+             => is_var s; intro a; move a at top; generalize dependent s;
+                  lazymatch goal with
+                  | [ |- forall s (a : op s tZ), @?P s a ]
+                    => intros s a;
+                         refine match a as a' in op s' d'
+                                      return match d' return op s' d' -> _ with
+                                             | tZ => fun a'' => P _ a''
+                                             | _ => fun _ => True
+                                             end a'
+                                with
+                                | OpConst _ _ => _
+                                | _ => _
+                                end;
+                         clear a;
+                         try exact I;
+                         intros
+                  end
+           | [ |- forall a : op ?s (tZ * tZ), @?P a ]
+             => is_var s; intro a; move a at top; generalize dependent s;
+                  lazymatch goal with
+                  | [ |- forall s (a : op s (tZ * tZ)), @?P s a ]
+                    => intros s a;
+                         refine match a as a' in op s' d'
+                                      return match d' return op s' d' -> _ with
+                                             | Prod tZ tZ => fun a'' => P _ a''
+                                             | _ => fun _ => True
+                                             end a'
+                                with
+                                | OpConst _ _ => _
+                                | _ => _
+                                end;
+                         clear a;
+                         try exact I;
+                         intros
+                  end
+           | [ |- forall e : exprf Unit, @?P e ]
+             => intro e;
+                  refine match e as e' in Named.exprf _ _ _ t
+                               return match t return exprf t -> _ with
+                                      | Unit => fun e' => P e'
+                                      | _ => fun _ => True
+                                      end e'
+                         with
+                         | TT => _
+                         | _ => _
+                         end;
+                  clear e;
+                  try exact I;
+                  intros
+           | [ |- forall e : exprf tZ, @?P e ]
+             => intro e;
+                  refine match e as e' in Named.exprf _ _ _ t
+                               return match t return exprf t -> _ with
+                                      | tZ => fun e' => P e'
+                                      | _ => fun _ => True
+                                      end e'
+                         with
+                         | TT => _
+                         | _ => _
+                         end;
+                  clear e;
+                  try exact I;
+                  intros
+           | [ |- forall e : exprf (tZ * tZ), @?P e ]
+             => intro e;
+                  refine match e as e' in Named.exprf _ _ _ t
+                               return match t return exprf t -> _ with
+                                      | (tZ * tZ)%ctype => fun e' => P e'
+                                      | _ => fun _ => True
+                                      end e'
+                         with
+                         | TT => _
+                         | _ => _
+                         end;
+                  clear e;
+                  try exact I;
+                  intros
+           | [ |- forall e : exprf (tZ * tZ * tZ), @?P e ]
+             => intro e;
+                  refine match e as e' in Named.exprf _ _ _ t
+                               return match t return exprf t -> _ with
+                                      | (tZ * tZ * tZ)%ctype => fun e' => P e'
+                                      | _ => fun _ => True
+                                      end e'
+                         with
+                         | TT => _
+                         | _ => _
+                         end;
+                  clear e;
+                  try exact I;
+                  intros
+     end.
+         solve [ repeat first [ t_step | t'_step ] ].
+             solve [ repeat first [ t_step | t'_step ] ].
+             match goal with
+           | [ H : context[match ?e with _ => _ end] |- _ = _ ]
+             => first [ is_var e; destruct e
+                      | revert dependent e ]
+           | [ |- context[match ?e with _ => _ end] ]
+             => first [ is_var e; destruct e
+                      | revert dependent e ]
+           | _ => exact I
+           | [ |- forall a : op ?s tZ, @?P a ]
+             => is_var s; intro a; move a at top; generalize dependent s;
+                  lazymatch goal with
+                  | [ |- forall s (a : op s tZ), @?P s a ]
+                    => intros s a;
+                         refine match a as a' in op s' d'
+                                      return match d' return op s' d' -> _ with
+                                             | tZ => fun a'' => P _ a''
+                                             | _ => fun _ => True
+                                             end a'
+                                with
+                                | OpConst _ _ => _
+                                | _ => _
+                                end;
+                         clear a;
+                         try exact I;
+                         intros
+                  end
+           | [ |- forall a : op ?s (tZ * tZ), @?P a ]
+             => is_var s; intro a; move a at top; generalize dependent s;
+                  lazymatch goal with
+                  | [ |- forall s (a : op s (tZ * tZ)), @?P s a ]
+                    => intros s a;
+                         refine match a as a' in op s' d'
+                                      return match d' return op s' d' -> _ with
+                                             | Prod tZ tZ => fun a'' => P _ a''
+                                             | _ => fun _ => True
+                                             end a'
+                                with
+                                | OpConst _ _ => _
+                                | _ => _
+                                end;
+                         clear a;
+                         try exact I;
+                         intros
+                  end
+           | [ |- forall e : exprf Unit, @?P e ]
+             => intro e;
+                  refine match e as e' in Named.exprf _ _ _ t
+                               return match t return exprf t -> _ with
+                                      | Unit => fun e' => P e'
+                                      | _ => fun _ => True
+                                      end e'
+                         with
+                         | TT => _
+                         | _ => _
+                         end;
+                  clear e;
+                  try exact I;
+                  intros
+           | [ |- forall e : exprf tZ, @?P e ]
+             => intro e;
+                  refine match e as e' in Named.exprf _ _ _ t
+                               return match t return exprf t -> _ with
+                                      | tZ => fun e' => P e'
+                                      | _ => fun _ => True
+                                      end e'
+                         with
+                         | TT => _
+                         | _ => _
+                         end;
+                  clear e;
+                  try exact I;
+                  intros
+           | [ |- forall e : exprf (tZ * tZ), @?P e ]
+             => intro e;
+                  refine match e as e' in Named.exprf _ _ _ t
+                               return match t return exprf t -> _ with
+                                      | (tZ * tZ)%ctype => fun e' => P e'
+                                      | _ => fun _ => True
+                                      end e'
+                         with
+                         | TT => _
+                         | _ => _
+                         end;
+                  clear e;
+                  try exact I;
+                  intros
+           | [ |- forall e : exprf (tZ * tZ * tZ), @?P e ]
+             => intro e;
+                  refine match e as e' in Named.exprf _ _ _ t
+                               return match t return exprf t -> _ with
+                                      | (tZ * tZ * tZ)%ctype => fun e' => P e'
+                                      | _ => fun _ => True
+                                      end e'
+                         with
+                         | TT => _
+                         | _ => _
+                         end;
+                  clear e;
+                  try exact I;
+                  intros
+             end.
+             2:
+             solve [ repeat first [ t_step | t'_step ] ].
+             match goal with
+           | [ H : context[match ?e with _ => _ end] |- _ = _ ]
+             => first [ is_var e; destruct e
+                      | revert dependent e ]
+           | [ |- context[match ?e with _ => _ end] ]
+             => first [ is_var e; destruct e
+                      | revert dependent e ]
+           | _ => exact I
+           | [ |- forall a : op ?s tZ, @?P a ]
+             => is_var s; intro a; move a at top; generalize dependent s;
+                  lazymatch goal with
+                  | [ |- forall s (a : op s tZ), @?P s a ]
+                    => intros s a;
+                         refine match a as a' in op s' d'
+                                      return match d' return op s' d' -> _ with
+                                             | tZ => fun a'' => P _ a''
+                                             | _ => fun _ => True
+                                             end a'
+                                with
+                                | OpConst _ _ => _
+                                | _ => _
+                                end;
+                         clear a;
+                         try exact I;
+                         intros
+                  end
+           | [ |- forall a : op ?s (tZ * tZ), @?P a ]
+             => is_var s; intro a; move a at top; generalize dependent s;
+                  lazymatch goal with
+                  | [ |- forall s (a : op s (tZ * tZ)), @?P s a ]
+                    => intros s a;
+                         refine match a as a' in op s' d'
+                                      return match d' return op s' d' -> _ with
+                                             | Prod tZ tZ => fun a'' => P _ a''
+                                             | _ => fun _ => True
+                                             end a'
+                                with
+                                | OpConst _ _ => _
+                                | _ => _
+                                end;
+                         clear a;
+                         try exact I;
+                         intros
+                  end
+           | [ |- forall e : exprf Unit, @?P e ]
+             => intro e;
+                  refine match e as e' in Named.exprf _ _ _ t
+                               return match t return exprf t -> _ with
+                                      | Unit => fun e' => P e'
+                                      | _ => fun _ => True
+                                      end e'
+                         with
+                         | TT => _
+                         | _ => _
+                         end;
+                  clear e;
+                  try exact I;
+                  intros
+           | [ |- forall e : exprf tZ, @?P e ]
+             => intro e;
+                  refine match e as e' in Named.exprf _ _ _ t
+                               return match t return exprf t -> _ with
+                                      | tZ => fun e' => P e'
+                                      | _ => fun _ => True
+                                      end e'
+                         with
+                         | TT => _
+                         | _ => _
+                         end;
+                  clear e;
+                  try exact I;
+                  intros
+           | [ |- forall e : exprf (tZ * tZ), @?P e ]
+             => intro e;
+                  refine match e as e' in Named.exprf _ _ _ t
+                               return match t return exprf t -> _ with
+                                      | (tZ * tZ)%ctype => fun e' => P e'
+                                      | _ => fun _ => True
+                                      end e'
+                         with
+                         | TT => _
+                         | _ => _
+                         end;
+                  clear e;
+                  try exact I;
+                  intros
+           | [ |- forall e : exprf (tZ * tZ * tZ), @?P e ]
+             => intro e;
+                  refine match e as e' in Named.exprf _ _ _ t
+                               return match t return exprf t -> _ with
+                                      | (tZ * tZ * tZ)%ctype => fun e' => P e'
+                                      | _ => fun _ => True
+                                      end e'
+                         with
+                         | TT => _
+                         | _ => _
+                         end;
+                  clear e;
+                  try exact I;
+                  intros
+             end.
+             2:
+               solve [ repeat first [ t_step | t'_step ] ].
+             2:
+               solve [ repeat first [ t_step | t'_step ] ].
+             break_innermost_match_hyps_step.
+             2:solve [ repeat first [ t_step | t'_step ] ].
+             2:solve [ repeat first [ t_step | t'_step ] ].
+             break_innermost_match_hyps_step.
+             2:solve [ repeat first [ t_step | t'_step ] ].
+             break_innermost_match_hyps_step.
+                          match goal with
+           | [ H : context[match ?e with _ => _ end] |- _ = _ ]
+             => first [ is_var e; destruct e
+                      | revert dependent e ]
+           | [ |- context[match ?e with _ => _ end] ]
+             => first [ is_var e; destruct e
+                      | revert dependent e ]
+           | _ => exact I
+           | [ |- forall a : op ?s tZ, @?P a ]
+             => is_var s; intro a; move a at top; generalize dependent s;
+                  lazymatch goal with
+                  | [ |- forall s (a : op s tZ), @?P s a ]
+                    => intros s a;
+                         refine match a as a' in op s' d'
+                                      return match d' return op s' d' -> _ with
+                                             | tZ => fun a'' => P _ a''
+                                             | _ => fun _ => True
+                                             end a'
+                                with
+                                | OpConst _ _ => _
+                                | _ => _
+                                end;
+                         clear a;
+                         try exact I;
+                         intros
+                  end
+           | [ |- forall a : op ?s (tZ * tZ), @?P a ]
+             => is_var s; intro a; move a at top; generalize dependent s;
+                  lazymatch goal with
+                  | [ |- forall s (a : op s (tZ * tZ)), @?P s a ]
+                    => intros s a;
+                         refine match a as a' in op s' d'
+                                      return match d' return op s' d' -> _ with
+                                             | Prod tZ tZ => fun a'' => P _ a''
+                                             | _ => fun _ => True
+                                             end a'
+                                with
+                                | OpConst _ _ => _
+                                | _ => _
+                                end;
+                         clear a;
+                         try exact I;
+                         intros
+                  end
+           | [ |- forall e : exprf Unit, @?P e ]
+             => intro e;
+                  refine match e as e' in Named.exprf _ _ _ t
+                               return match t return exprf t -> _ with
+                                      | Unit => fun e' => P e'
+                                      | _ => fun _ => True
+                                      end e'
+                         with
+                         | TT => _
+                         | _ => _
+                         end;
+                  clear e;
+                  try exact I;
+                  intros
+           | [ |- forall e : exprf tZ, @?P e ]
+             => intro e;
+                  refine match e as e' in Named.exprf _ _ _ t
+                               return match t return exprf t -> _ with
+                                      | tZ => fun e' => P e'
+                                      | _ => fun _ => True
+                                      end e'
+                         with
+                         | TT => _
+                         | _ => _
+                         end;
+                  clear e;
+                  try exact I;
+                  intros
+           | [ |- forall e : exprf (tZ * tZ), @?P e ]
+             => intro e;
+                  refine match e as e' in Named.exprf _ _ _ t
+                               return match t return exprf t -> _ with
+                                      | (tZ * tZ)%ctype => fun e' => P e'
+                                      | _ => fun _ => True
+                                      end e'
+                         with
+                         | TT => _
+                         | _ => _
+                         end;
+                  clear e;
+                  try exact I;
+                  intros
+           | [ |- forall e : exprf (tZ * tZ * tZ), @?P e ]
+             => intro e;
+                  refine match e as e' in Named.exprf _ _ _ t
+                               return match t return exprf t -> _ with
+                                      | (tZ * tZ * tZ)%ctype => fun e' => P e'
+                                      | _ => fun _ => True
+                                      end e'
+                         with
+                         | TT => _
+                         | _ => _
+                         end;
+                  clear e;
+                  try exact I;
+                  intros
+             end.
+             do 2 match goal with
+           | [ H : context[match ?e with _ => _ end] |- _ = _ ]
+             => first [ is_var e; destruct e
+                      | revert dependent e ]
+           | [ |- context[match ?e with _ => _ end] ]
+             => first [ is_var e; destruct e
+                      | revert dependent e ]
+           | _ => exact I
+           | [ |- forall a : op ?s tZ, @?P a ]
+             => is_var s; intro a; move a at top; generalize dependent s;
+                  lazymatch goal with
+                  | [ |- forall s (a : op s tZ), @?P s a ]
+                    => intros s a;
+                         refine match a as a' in op s' d'
+                                      return match d' return op s' d' -> _ with
+                                             | tZ => fun a'' => P _ a''
+                                             | _ => fun _ => True
+                                             end a'
+                                with
+                                | OpConst _ _ => _
+                                | _ => _
+                                end;
+                         clear a;
+                         try exact I;
+                         intros
+                  end
+           | [ |- forall a : op ?s (tZ * tZ), @?P a ]
+             => is_var s; intro a; move a at top; generalize dependent s;
+                  lazymatch goal with
+                  | [ |- forall s (a : op s (tZ * tZ)), @?P s a ]
+                    => intros s a;
+                         refine match a as a' in op s' d'
+                                      return match d' return op s' d' -> _ with
+                                             | Prod tZ tZ => fun a'' => P _ a''
+                                             | _ => fun _ => True
+                                             end a'
+                                with
+                                | OpConst _ _ => _
+                                | _ => _
+                                end;
+                         clear a;
+                         try exact I;
+                         intros
+                  end
+           | [ |- forall e : exprf Unit, @?P e ]
+             => intro e;
+                  refine match e as e' in Named.exprf _ _ _ t
+                               return match t return exprf t -> _ with
+                                      | Unit => fun e' => P e'
+                                      | _ => fun _ => True
+                                      end e'
+                         with
+                         | TT => _
+                         | _ => _
+                         end;
+                  clear e;
+                  try exact I;
+                  intros
+           | [ |- forall e : exprf tZ, @?P e ]
+             => intro e;
+                  refine match e as e' in Named.exprf _ _ _ t
+                               return match t return exprf t -> _ with
+                                      | tZ => fun e' => P e'
+                                      | _ => fun _ => True
+                                      end e'
+                         with
+                         | TT => _
+                         | _ => _
+                         end;
+                  clear e;
+                  try exact I;
+                  intros
+           | [ |- forall e : exprf (tZ * tZ), @?P e ]
+             => intro e;
+                  refine match e as e' in Named.exprf _ _ _ t
+                               return match t return exprf t -> _ with
+                                      | (tZ * tZ)%ctype => fun e' => P e'
+                                      | _ => fun _ => True
+                                      end e'
+                         with
+                         | TT => _
+                         | _ => _
+                         end;
+                  clear e;
+                  try exact I;
+                  intros
+           | [ |- forall e : exprf (tZ * tZ * tZ), @?P e ]
+             => intro e;
+                  refine match e as e' in Named.exprf _ _ _ t
+                               return match t return exprf t -> _ with
+                                      | (tZ * tZ * tZ)%ctype => fun e' => P e'
+                                      | _ => fun _ => True
+                                      end e'
+                         with
+                         | TT => _
+                         | _ => _
+                         end;
+                  clear e;
+                  try exact I;
+                  intros
+                  end.
+             solve [ repeat first [ t_step | t'_step ] ].
+             solve [ repeat first [ t_step | t'_step ] ].
+             solve [ repeat first [ t_step | t'_step ] ].
+             break_innermost_match_step.
+             solve [ repeat first [ t_step | t'_step ] ].
+             solve [ repeat first [ t_step | t'_step ] ].
+             { break_innermost_match_step.
+               2:solve [ repeat first [ t_step | t'_step ] ].
+               2:solve [ repeat first [ t_step | t'_step ] ].
+               break_innermost_match_step.
+               2:solve [ repeat first [ t_step | t'_step ] ].
+               break_innermost_match_step.
+               2:solve [ repeat first [ t_step | t'_step ] ].
+               2:solve [ repeat first [ t_step | t'_step ] ].
+               break_innermost_match_step.
+               2:solve [ repeat first [ t_step | t'_step ] ].
+               Local Ltac t := match goal with
+           | [ H : context[match ?e with _ => _ end] |- _ = _ ]
+             => first [ is_var e; destruct e
+                      | revert dependent e ]
+           | [ |- context[match ?e with _ => _ end] ]
+             => first [ is_var e; destruct e
+                      | revert dependent e ]
+           | _ => exact I
+           | [ |- forall a : op ?s tZ, @?P a ]
+             => is_var s; intro a; move a at top; generalize dependent s;
+                  lazymatch goal with
+                  | [ |- forall s (a : op s tZ), @?P s a ]
+                    => intros s a;
+                         refine match a as a' in op s' d'
+                                      return match d' return op s' d' -> _ with
+                                             | tZ => fun a'' => P _ a''
+                                             | _ => fun _ => True
+                                             end a'
+                                with
+                                | OpConst _ _ => _
+                                | _ => _
+                                end;
+                         clear a;
+                         try exact I;
+                         intros
+                  end
+           | [ |- forall a : op ?s (tZ * tZ), @?P a ]
+             => is_var s; intro a; move a at top; generalize dependent s;
+                  lazymatch goal with
+                  | [ |- forall s (a : op s (tZ * tZ)), @?P s a ]
+                    => intros s a;
+                         refine match a as a' in op s' d'
+                                      return match d' return op s' d' -> _ with
+                                             | Prod tZ tZ => fun a'' => P _ a''
+                                             | _ => fun _ => True
+                                             end a'
+                                with
+                                | OpConst _ _ => _
+                                | _ => _
+                                end;
+                         clear a;
+                         try exact I;
+                         intros
+                  end
+           | [ |- forall e : exprf Unit, @?P e ]
+             => intro e;
+                  refine match e as e' in Named.exprf _ _ _ t
+                               return match t return exprf t -> _ with
+                                      | Unit => fun e' => P e'
+                                      | _ => fun _ => True
+                                      end e'
+                         with
+                         | TT => _
+                         | _ => _
+                         end;
+                  clear e;
+                  try exact I;
+                  intros
+           | [ |- forall e : exprf tZ, @?P e ]
+             => intro e;
+                  refine match e as e' in Named.exprf _ _ _ t
+                               return match t return exprf t -> _ with
+                                      | tZ => fun e' => P e'
+                                      | _ => fun _ => True
+                                      end e'
+                         with
+                         | TT => _
+                         | _ => _
+                         end;
+                  clear e;
+                  try exact I;
+                  intros
+           | [ |- forall e : exprf (tZ * tZ), @?P e ]
+             => intro e;
+                  refine match e as e' in Named.exprf _ _ _ t
+                               return match t return exprf t -> _ with
+                                      | (tZ * tZ)%ctype => fun e' => P e'
+                                      | _ => fun _ => True
+                                      end e'
+                         with
+                         | TT => _
+                         | _ => _
+                         end;
+                  clear e;
+                  try exact I;
+                  intros
+           | [ |- forall e : exprf (tZ * tZ * tZ), @?P e ]
+             => intro e;
+                  refine match e as e' in Named.exprf _ _ _ t
+                               return match t return exprf t -> _ with
+                                      | (tZ * tZ * tZ)%ctype => fun e' => P e'
+                                      | _ => fun _ => True
+                                      end e'
+                         with
+                         | TT => _
+                         | _ => _
+                         end;
+                  clear e;
+                  try exact I;
+                  intros
+                               end.
+               t.
+               t.
+               break_innermost_match_step.
+               2:solve [ repeat first [ t_step | t'_step ] ].
+               break_innermost_match_step.
+               2:solve [ repeat first [ t_step | t'_step ] ].
+               break_innermost_match_step.
+               2:solve [ repeat first [ t_step | t'_step ] ].
+               2:solve [ repeat first [ t_step | t'_step ] ].
+               2:solve [ repeat first [ t_step | t'_step ] ].
+               2:solve [ repeat first [ t_step | t'_step ] ].
+               2:solve [ repeat first [ t_step | t'_step ] ].
+               2:solve [ repeat first [ t_step | t'_step ] ].
+             solve [ repeat first [ t_step | t'_step ] ].
+             brea
+             solve [ repeat first [ t_step | t'_step ] ].
+             2:solve [ repeat first [ t_step | t'_step ] ].
+             2:solve [ repeat first [ t_step | t'_step ] ].
+             Focus 9.
+
+             2:
+             solve [ repeat first [ t_step | t'_step ] ].
+               | revert dependent e ]
+    end
+    shelve.
+    solve [ repeat first [ t_step | t'_step ] ].
+    solve [ repeat first [ t_step | t'_step ] ].
+    solve [ repeat first [ t_step | t'_step ] ].
+    solve [ repeat first [ t_step | t'_step ] ].
+    solve [ repeat first [ t_step | t'_step ] ].
+    solve [ repeat first [ t_step | t'_step ] ].
+    solve [ repeat first [ t_step | t'_step ] ].
+    solve [ repeat first [ t_step | t'_step ] ].
+    solve [ repeat first [ t_step | t'_step ] ].
+    solve [ repeat first [ t_step | t'_step ] ].
+    solve [ repeat first [ t_step | t'_step ] ].
+    solve [ repeat first [ t_step | t'_step ] ].
+    solve [ repeat first [ t_step | t'_step ] ].
+    solve [ repeat first [ t_step | t'_step ] ].
+    solve [ repeat first [ t_step | t'_step ] ].
+    solve [ repeat first [ t_step | t'_step ] ].
+    solve [ repeat first [ t_step | t'_step ] ].
+    solve [ repeat first [ t_step | t'_step ] ].
+    solve [ repeat first [ t_step | t'_step ] ].
+    solve [ repeat first [ t_step | t'_step ] ].
+    solve [ repeat first [ t_step | t'_step ] ].
+    solve [ repeat first [ t_step | t'_step ] ].
+    solve [ repeat first [ t_step | t'_step ] ].
+    solve [ repeat first [ t_step | t'_step ] ].
+    solve [ repeat first [ t_step | t'_step ] ].
+    solve [ repeat first [ t_step | t'_step ] ].
+    solve [ repeat first [ t_step | t'_step ] ].
+    solve [ repeat first [ t_step | t'_step ] ].
+    solve [ repeat first [ t_step | t'_step ] ].
+    solve [ repeat first [ t_step | t'_step ] ].
+    solve [ repeat first [ t_step | t'_step ] ].
+    solve [ repeat first [ t_step | t'_step ] ].
+    solve [ repeat first [ t_step | t'_step ] ].
+    solve [ repeat first [ t_step | t'_step ] ].
+    solve [ repeat first [ t_step | t'_step ] ].
+    solve [ repeat first [ t_step | t'_step ] ].
+    solve [ repeat first [ t_step | t'_step ] ].
+    solve [ repeat first [ t_step | t'_step ] ].
+    solve [ repeat first [ t_step | t'_step ] ].
+    solve [ repeat first [ t_step | t'_step ] ].
+    solve [ repeat first [ t_step | t'_step ] ].
+    solve [ repeat first [ t_step | t'_step ] ].
+    solve [ repeat first [ t_step | t'_step ] ].
+    solve [ repeat first [ t_step | t'_step ] ].
+    Unshelve.
+    Focus 2.
+    { repeat first [ t_step | t'_step ].
+      Arguments interpf : clear implicits.
+    Focus 2.
+    revert dependent o.
+    match goal with
+    end.
+    break_innermost_match_step.
+    break_innermost_match_step.
+    intros.
+    break_innermost_match_hyps_step.
+    break_innermost_match_hyps_step.
+    break_innermost_match_hyps_step.
+    revert dependent e0.
+    match goal with
+    end.
+    break_innermost_match_step; try exact I.
+    break_innermost_match_step; try exact I.
+    solve [ repeat first [ t_step | t'_step ] ].
+    solve [ repeat first [ t_step | t'_step ] ].
+    { break_innermost_match_step; try exact I.
+      break_innermost_match_step; try exact I.
+      break_innermost_match_step; try exact I.
+      break_innermost_match_step; try exact I.
+      break_innermost_match_step; try exact I.
+      break_innermost_match_step; try exact I.
+      break_innermost_match_step; try exact I.
+      intros.
+      revert dependent e3.
+      match goal with
+      | [ |- forall e : exprf (tZ * tZ), @?P e ]
+        => intro e;
+             refine match e as e' in Named.exprf _ _ _ t
+                          return match t return exprf t -> _ with
+                                 | (tZ * tZ)%ctype => fun e' => P e'
+                                 | _ => fun _ => True
+                                 end e'
+                    with
+                    | TT => _
+                    | _ => _
+                    end;
+             clear e;
+             try exact I;
+             intros
+      end.
+      solve [ repeat first [ t_step | t'_step ] ].
+    { break_innermost_match_step; try exact I.
+      break_innermost_match_step; try exact I.
+      break_innermost_match_step; try exact I.
+      break_innermost_match_step; try exact I.
+      break_innermost_match_step; try exact I.
+      solve [ repeat first [ t_step | t'_step ] ]. }
+    { break_innermost_match_step; try exact I.
+      break_innermost_match_step; try exact I.
+      break_innermost_match_step; try exact I.
+      break_innermost_match_step; try exact I.
+      break_innermost_match_step; try exact I.
+      intros.
+      revert dependent e0.
+      match goal with
+      end.
+      solve [ repeat first [ t_step | t'_step ] ].
+      solve [ repeat first [ t_step | t'_step ] ].
+      break_innermost_match_step; try exact I.
+      break_innermost_match_step; try exact I.
+      solve [ repeat first [ t_step | t'_step ] ].
+      intros.
+      solve [ repeat first [ t_step | t'_step ] ].
+
+    solve [ repeat first [ t_step | t'_step ] ].
+
+
+      break_innermost_match_step; try exact I.
+      break_innermost_match_step; try exact I.
+    {
+    | [ |- forall a : op ?s (tZ * tZ), @?P a ]
+      => is_var s; intro a; move a at top; generalize dependent s;
+         lazymatch goal with
+         | [ |- forall s (a : op s (tZ * tZ)), @?P s a ]
+           => intros s a;
+                refine match a as a' in op s' d'
+                             return match d' return op s' d' -> _ with
+                                    | Prod tZ tZ => fun a'' => P _ a''
+                                    | _ => fun _ => True
+                                    end a'
+                       with
+                       | OpConst _ _ => _
+                       | _ => _
+                       end;
+                clear a;
+                try exact I;
+                intros
+         end
+    end.
+    break_innermost_match_step.
+
+
+    match goal with
+    | [ |- forall a : op _ _, @?P a ]
+      => intro a; refine match a in op s d as a' return P a' with
+                         | OpConst _ _ => _
+                         | _ => _
+                         end; clear a
+    end.
+    {
+      refine match o with
+             | OpConst _ _ => _
+             | _ => _
+             end.
+      solve [ repeat first [ t_step | t'_step ] ].
+      solve [ repeat first [ t_step | t'_step ] ].
+      solve [ repeat first [ t_step | t'_step ] ].
+      solve [ repeat first [ t_step | t'_step ] ].
+      solve [ repeat first [ t_step | t'_step ] ].
+      solve [ repeat first [ t_step | t'_step ] ].
+      solve [ repeat first [ t_step | t'_step ] ].
+      solve [ repeat first [ t_step | t'_step ] ].
+      solve [ repeat first [ t_step | t'_step ] ].
+      solve [ repeat first [ t_step | t'_step ] ].
+      solve [ repeat first [ t_step | t'_step ] ].
+      break_innermost_match_step.
+      break_innermost_match_step.
+    solve [ repeat first [ t_step | t'_step ] ].
+    Focus 3.
+    Focus 2.
+    Focus 2.
+    match goal with
+    | [
+    2:repeat first [ t_step | t'_step ].
+    { repeat t_step.
+      t_destruct_step.
+      { repeat first [ t_step | t'_step | t_invert_step ]. }
+      { repeat first [ t_step | t'_step | t_invert_step ]. }
+      { t_destruct_step.
+        { repeat first [ t_step | t'_step | t_invert_step ]. }
+        { repeat first [ t_step | t'_step ]. }
+        { repeat first [ t_step | t'_step ]. }
+        { repeat first [ t_step | t'_step ]. }
+        { repeat first [ t_step | t'_step ]. }
+        { repeat first [ t_step | t'_step ]. }
+        { repeat first [ t_step | t'_step ]. }
+        { repeat first [ t_step | t'_step ]. }
+        { repeat first [ t_step | t'_step ]. }
+        { repeat first [ t_step | t'_step ]. }
+        { repeat first [ t_step | t'_step ]. }
+        { move Tout1 at bottom.
+          destruct Tout1, Tout2.
+          repeat t_step.
+          { invert_expr.
+            Set Printing Depth 100000.
+            { t_destruct_step; repeat t_step. }
+            Focus 2.
+            break_innermost_match; try exact I; intros.
+            { repeat t_step. }
+            { repeat first [ t_step | t'_step ]. }
+            { repeat t_step. }
+            { repeat t_step. }
+            { repeat t_step. }
+            { repeat t_step. }
+            { repeat t_step. }
+            { repeat t_step. }
+            { repeat t_step. }
+            { repeat t_step. }
+            { repeat t_step. }
+            { repeat t_step. }
+            { repeat t_step. }
+            { repeat t_step. }
+            { repeat t_step. }
+            { repeat t_step. }
+            { repeat t_step. }
+            { repeat t_step. }
+            { repeat t_step. }
+            { repeat t_step. }
+            all:try exact I.
+            2:solve [ t_destruct_step; repeat t_step ].
+            { t_destruct_step; repeat t_step.
+              { t_destruct_step; repeat t_step. }
+              { t_destruct_step; repeat t_step.
+                { t_destruct_step; repeat t_step. }
+                { repeat first [ t_step | t'_step ]. }
+                { repeat first [ t_step | t'_step ]. } }
+              { repeat first [ t_step | t'_step ]. } }
+            { t_destruct_step; repeat t_step.
+
+
+                { repeat first [ t_step | t'_step ]. }
+                { repeat first [ t_step | t'_step ]. }
+                { repeat first [ t_step | t'_step ]. }
+              { t_destruct_step; repeat t_step.
+
+                { repeat first [ t_step | t'_step ]. }
+              { repeat first [ t_step | t'_step ]. }
+                { repeat first [ t_step | t'_step ]. }
+                  Arguments interpf : clear implicits.
+                  move IHe2 at bottom.
+                  move H at bottom.
+                  specialize (fun v2 => IHe2 _ v2 H).
+                { t_destruct_step; repeat t_step.
+                  { t_destruct_step; repeat t_step. }
+                  { t_destruct_step; repeat t_step.
+                    { t_destruct_step; repeat t_step. }
+                    { t_destruct_step; repeat t_step.
+                      { t_destruct_step; repeat t_step. }
+                      { t_destruct_step; repeat t_step.
+                        { t_destruct_step; repeat t_step. }
+                        Set Printing Depth 1000000.
+                        {
+                  } } }
+
+                    { t_destruct_step; repeat t_step. } } }
+              t_destruct_step; repeat t_step.
+              t_destruct_step; repeat t_step.
+              t_destruct_step; repeat t_step.
+              { t_destruct_step; repeat t_step.
+              t_destruct_step; repeat t_step.
+              t_destruct_step; repeat t_step.
+              t_destruct_step; repeat t_step.
+              t_destruct_step; repeat t_step.
+              t_destruct_step; repeat t_step.
+              break_innermost_match_step; try exact I.
+            all:break_innermost_match_step; try exact I.
+            { repeat first [ t_step | t'_step ].
+
+            }
+            { repeat first [ t_step | t'_step ]. }
+          t_destruct_step.
+        { simpl in *.
+          repeat t_step.
+          t'_step.
+          repeat t_step.
+          t'_step.
+          repeat t_step.
+          repeat t_step.
+          repeat t_step.
+          match goal with
+          end.
+          match goal with
+          end.
+          Set Printing Implicit.
+          t'_step.
+          repeat t_step.
+          rewrite H in IHe2.
+          t'_step.
+          repeat t_step.
+          t'_step.
+          repeat t_step.
+          { match goal with
+            end.
+          repeat first [ t_step | t'_step ]. }
+      Focus 4.
+
+      simpl.
+      .
+
+             try first [ break_innermost_match_hyps_step
+                       | progress invert_expr; break_innermost_match; try exact I; intros ]).
+    { clear -H0.
+
+      invert_one_expr e1.
+      do 20 (repeat first [ progress simpl in *
+                   | reflexivity
+                   | congruence
+                   | progress unfold option_map, LetIn.Let_In in *
+                   | progress intros
+                   | progress subst
+                   | progress inversion_option
+                   | progress destruct_head' unit
+                   | solve [ f_equal; eauto ]
+                   | match goal with
+                     | [ H : interpf ?e = Some ?v, H' : interpf (rewrite_exprf ?e') = Some ?v' |- _ ]
+                       => assert (v = v') by eauto; subst v
+                     end
+                   | break_innermost_match_step ];
+              first [ break_innermost_match_hyps_step
+                    | progress invert_expr; break_innermost_match; try exact I; intros ]).
+      progress invert_expr.
+             .
+    {
+      do 10 (repeat first [ progress simpl in *
+                   | reflexivity
+                   | congruence
+                   | progress unfold option_map, LetIn.Let_In in *
+                   | progress intros
+                   | progress subst
+                   | progress inversion_option
+                   | solve [ f_equal; eauto ]
+                   | match goal with
+                     | [ H : interpf ?e = Some ?v, H' : interpf (rewrite_exprf ?e') = Some ?v' |- _ ]
+                       => assert (v = v') by eauto; subst v
+                     end
+                   | break_innermost_match_step ];
+             try break_innermost_match_hyps_step).
+    Focus 9.
+    Focus 2.
+    { .
+      repeat first [ progress simpl in *
+                   | reflexivity
+                   | congruence
+                   | progress unfold option_map, LetIn.Let_In in *
+                   | progress intros
+                   | progress subst
+                   | progress inversion_option
+                   | solve [ f_equal; eauto ]
+                   | break_innermost_match_step ].
+    Focus 2.
+    { break_innermost_match_hyps;
+      repeat first [ progress simpl in *
+                   | reflexivity
+                   | congruence
+                   | progress unfold option_map in *
+                   | progress intros
+                   | progress subst
+                   | progress inversion_option
+                   | solve [ f_equal; eauto ]
+                   | break_innermost_match_step ]. }
+    Unfocus.
+    break_innermost_match_hyps_step.
+      f_equal; eauto.
+
+
+        do_rewrite
+             (rewrite_exprf : forall t (e : exprf t), exprf t)
+             {t} (e : exprf t)
+    : exprf t
+    := match e in Named.exprf _ _ _ t return exprf t with
+       |           (nlet (a2, c1) : tZ * tZ := (ADD bw1 a b as ex0) in P0)
+         => match rewrite_exprf _ P0 in Named.exprf _ _ _ t return exprf t -> exprf t with
+            |      (nlet (s , c2) : tZ * tZ := (ADD bw2 c0 (Var _ a2') as ex1) in P1)
+              => match P1 in Named.exprf _ _ _ t return exprf t -> exprf t with
+                 | (nlet c        : tZ      := (ADX (Var _ c1') (Var _ c2') as ex2) in P)
+                   => fun e
+                      => if (((bw1 =Z? bw2) && (a2 =n? a2') && (c1 =n? c1') && (c2 =n? c2'))
+                               && (is_const_or_var c0 && is_const_or_var a && is_const_or_var b)
+                               && negb (name_list_has_duplicate (a2::c1::s::c2::c::nil ++ get_namesf c0 ++ get_namesf a ++ get_namesf b)%list))
+                         then (nlet (a2, c1) : tZ * tZ := ex0 in
+                               nlet (s , c2) : tZ * tZ := ex1 in
+                               nlet c        : tZ      := ex2 in
+                               nlet (s, c)   : tZ * tZ := ADC bw1 c0 a b in
+                               P)
+                         else e
+                 | P1' => fun e => e
+                 end
+            | P0' => fun e => e
+            end (nlet (a2, c1) : tZ * tZ := rewrite_exprf _ ex0 in rewrite_exprf _ P0)
+       | TT => TT
+       | Var _ n => Var n
+       | Op _ _ opc args
+         => Op opc (rewrite_exprf _ args)
+       | (nlet nx := ex in eC)
+         => (nlet nx := rewrite_exprf _ ex in rewrite_exprf _ eC)
+       | Pair tx ex ty ey
+         => Pair (rewrite_exprf tx ex) (rewrite_exprf ty ey)
+       end%core%nexpr%bool.
+
+  Fixpoint rewrite_exprf {t} (e : exprf t) : exprf t
+    := @do_rewrite (@rewrite_exprf) t e.
+
+  Definition rewrite_expr {t} (e : expr t) : expr t
+    := match e in Named.expr _ _ _ t return expr t with
+       | Abs _ _ n f => Abs n (rewrite_exprf f)
+       end.
+End named.
+
+
+interp_base_type : base_type -> Type
+  interp_op : forall src dst : flat_type base_type,
+              op src dst ->
+              interp_flat_type interp_base_type src -> interp_flat_type interp_base_type dst
+  t : type base_type
+  e : Expr base_type op t
+  Hwf : Wf e
+  x : interp_flat_type interp_base_type
+        match (domain t -> codomain t)%ctype with
+        | x -> _ => x
+        end
+  e0 : Syntax.Named.expr base_type op BinNums.positive t
+  Heqo : Compile.compile (e (fun _ : base_type => BinNums.positive)) (Defaults.DefaultNamesFor e) =
+         Some e0
+  Heqo0 : Wf.Named.wf_unit Context.empty (RewriteAddToAdc.rewrite_expr positive_beq e0) =
+          Some PointedProp.trivial
+  e1 : Syntax.Named.expr base_type op FMapPositive.PositiveMap.key t
+  Heqo1 : DeadCodeElimination.EliminateDeadCode (RewriteAddToAdc.rewrite_expr positive_beq e0)
+            (Defaults.Named.default_names_for (RewriteAddToAdc.rewrite_expr positive_beq e0)) =
+          Some e1
+  Heqo2 : Wf.Named.wf_unit Context.empty e1 = Some PointedProp.trivial
+  H, H0 : true = true
+  i : interp_flat_type interp_base_type (codomain t)
+  Heqo3 : Syntax.Named.interp e1 x = Some i
+  i0 : interp_flat_type interp_base_type (codomain t)
+  Heqo4 : Syntax.Named.Interp (RewriteAddToAdc.rewrite_expr positive_beq e0) x = Some i0
+  ============================
+  i0 = Interp interp_op e x*)
+  Admitted.
+
+  Lemma interpf_do_rewriteo
+        {t} {e : exprf t}
+    : retT e (do_rewriteo e).
+  Proof.
+    unfold do_rewriteo; intros *; break_innermost_match; try congruence.
+    apply interpf_do_rewrite; assumption.
+  Qed.
+
+  Local Opaque RewriteAddToAdc.do_rewriteo.
+  Lemma interpf_rewrite_exprf
+        {t} (e : exprf t)
+    : retT e (rewrite_exprf e).
+  Proof.
+    pose t as T.
+    pose (rewrite_exprf_prestep (@rewrite_exprf) e) as E.
+    induction e; simpl in *;
+      intros ctx v H;
+      pose proof (interpf_do_rewriteo (t:=T) (e:=E) ctx v H); clear H;
+      subst T E;
+      repeat first [ assumption
+                   | progress unfold option_map, Let_In in *
+                   | progress simpl in *
+                   | progress subst
+                   | progress inversion_option
+                   | apply (f_equal (@Some _))
+                   | break_innermost_match_step
+                   | break_innermost_match_hyps_step
+                   | congruence
+                   | solve [ eauto ]
+                   | match goal with
+                     | [ IH : forall ctx v, interpf ?e = Some v -> _ = Some _, H' : interpf ?e = Some _ |- _ ]
+                       => specialize (IH _ _ H')
+                     | [ H : ?x = Some ?a, H' : ?x = Some ?b |- _ ]
+                       => assert (a = b) by congruence; (subst a || subst b)
+                     | [ |- ?rhs = Some _ ]
+                       => lazymatch rhs with
+                          | Some _ => fail
+                          | None => fail
+                          | _ => destruct rhs eqn:?
+                          end
+                     end ].
+  Qed.
+
+  Lemma interp_rewrite_expr
+        {t} (e : expr t)
+    : forall (ctx : InterpContext)
+             v x,
+      Named.interp (interp_op:=interp_op) (ctx:=ctx) (rewrite_expr e) x = Some v
+      -> Named.interp (interp_op:=interp_op) (ctx:=ctx) e x = Some v.
+  Proof.
+    unfold Named.interp, rewrite_expr; destruct e; simpl.
+    intros *; apply interpf_rewrite_exprf.
+  Qed.
+
+  Lemma Interp_rewrite_expr
+        {t} (e : expr t)
+    : forall v x,
+      Named.Interp (Context:=InterpContext) (interp_op:=interp_op) (rewrite_expr e) x = Some v
+      -> Named.Interp (Context:=InterpContext) (interp_op:=interp_op) e x = Some v.
+  Proof.
+    intros *; apply interp_rewrite_expr.
+  Qed.
+End named.
