src/Compilers/Z/RewriteAddToAdcInterp.v
@@ -1,0 +1,107 @@
+Require Import Crypto.Compilers.Named.PositiveContext.
+Require Import Crypto.Compilers.Named.ContextDefinitions.
+Require Import Crypto.Compilers.Named.InterpretToPHOASInterp.
+Require Import Crypto.Compilers.Named.CompileWf.
+Require Import Crypto.Compilers.Named.CompileInterp.
+Require Import Crypto.Compilers.Named.WfFromUnit.
+Require Import Crypto.Compilers.Named.DeadCodeEliminationInterp.
+Require Import Crypto.Compilers.Named.WfInterp.
+Require Import Crypto.Compilers.Syntax.
+Require Import Crypto.Compilers.Wf.
+Require Import Crypto.Compilers.Z.Syntax.
+Require Import Crypto.Compilers.Z.RewriteAddToAdc.
+Require Import Crypto.Compilers.Z.Named.RewriteAddToAdcInterp.
+Require Import Crypto.Util.Tactics.BreakMatch.
+Require Import Crypto.Util.Decidable.
+Require Import Crypto.Util.Bool.
+
+Section language.
+  Local Notation PContext var := (PositiveContext _ var _ internal_base_type_dec_bl).
+
+  Lemma InterpRewriteAdc
+        {interp_base_type}
+        {interp_op : forall src dst, op src dst -> interp_flat_type interp_base_type src -> interp_flat_type interp_base_type dst}
+        {t} (e : Expr base_type op t) (Hwf : Wf e)
+  : forall x, Interp interp_op (RewriteAdc e) x = Interp interp_op e x.
+  Proof.
+    intro x; unfold RewriteAdc, option_map; break_innermost_match; try reflexivity;
+      match goal with |- ?x = ?y => cut (Some x = Some y); [ congruence | ] end;
+      (etransitivity; [ symmetry; eapply @Interp_InterpToPHOAS | ]); try solve [
+      repeat first [ intros; eapply @PositiveContextOk
+                   | progress split_andb
+                   | congruence
+                   | tauto
+                   | solve [ auto | eapply @BinPos.Pos.eqb_eq; auto ]
+                   | eapply @Wf_from_unit
+                   | eapply @dec_rel_of_bool_dec_rel
+                   | eapply @internal_base_type_dec_lb
+                   | eapply @internal_base_type_dec_bl
+                   | eapply @InterpEliminateDeadCode; [ .. | eassumption | eassumption | ]
+                   | progress intros
+                   | rewrite !@lookupb_empty
+                   | eapply @wf_from_unit with (uContext:=PContext _); [ .. | eassumption ]
+                   | lazymatch goal with
+                     | [ |- Some _ = Some _ ] => fail
+                     | [ |- None = Some _ ] => exfalso; eapply @wf_interp_not_None; [ .. | unfold Syntax.Named.Interp in *; eassumption ]
+                     | [ |- ?x = Some _ ] => destruct x eqn:?; [ apply f_equal | ]
+                     end ] ].
+    { lazymatch goal with
+      | [ H : DeadCodeElimination.EliminateDeadCode _ _ = Some ?e |- Syntax.Named.Interp ?e _ = Some _ ]
+        => let lhs := match goal with |- ?lhs = _ => lhs end in
+           let v := fresh in
+           destruct lhs as [v|] eqn:?; [ apply f_equal; eapply @InterpEliminateDeadCode; [ .. | eassumption | try eassumption | try eassumption ]; clear H | ]
+      end;
+        try solve [       repeat first [ intros; eapply @PositiveContextOk
+                                       | eassumption
+                   | progress split_andb
+                   | congruence
+                   | tauto
+                   | solve [ auto | eapply @BinPos.Pos.eqb_eq; auto ]
+                   | eapply @Wf_from_unit
+                   | eapply @dec_rel_of_bool_dec_rel
+                   | eapply @internal_base_type_dec_lb
+                   | eapply @internal_base_type_dec_bl
+                   | eapply @InterpEliminateDeadCode; [ .. | eassumption | eassumption | ]
+                   | progress intros
+                   | rewrite !@lookupb_empty
+                   | eapply @wf_from_unit with (uContext:=PContext _); [ .. | eassumption ]
+                   | lazymatch goal with
+                     | [ |- Some _ = Some _ ] => fail
+                     | [ |- None = Some _ ] => exfalso; eapply @wf_interp_not_None; [ .. | unfold Syntax.Named.Interp in *; eassumption ]
+                     | [ |- ?x = Some _ ] => destruct x eqn:?; [ apply f_equal | ]
+                     end ] ].
+      lazymatch goal with
+      | [ H : DeadCodeElimination.EliminateDeadCode _ _ = Some ?e |- Syntax.Named.Interp ?e _ = Some _ ]
+        => let lhs := match goal with |- ?lhs = _ => lhs end in
+           let v := fresh in
+           destruct lhs as [v|] eqn:?; [ apply f_equal; eapply @InterpEliminateDeadCode; [ .. | eassumption | try eassumption | try eassumption ]; clear H | ]
+      | [ |- Syntax.Named.Interp (RewriteAddToAdc.rewrite_expr _ ?e) _ = Some _ ]
+        => let lhs := match goal with |- ?lhs = _ => lhs end in
+           let H := fresh in
+           destruct lhs eqn:H; [ apply (f_equal (@Some _)); eapply @Interp_rewrite_expr in H | ]
+      end;
+        try solve [       repeat first [ intros; eapply @PositiveContextOk
+                                       | eassumption
+                   | progress split_andb
+                   | congruence
+                   | tauto
+                   | solve [ auto | eapply @BinPos.Pos.eqb_eq; auto ]
+                   | eapply @Wf_from_unit
+                   | eapply @dec_rel_of_bool_dec_rel
+                   | eapply @internal_base_type_dec_lb
+                   | eapply @internal_base_type_dec_bl
+                   | eapply @InterpEliminateDeadCode; [ .. | eassumption | eassumption | ]
+                   | progress intros
+                   | rewrite !@lookupb_empty
+                   | eapply @wf_from_unit with (uContext:=PContext _); [ .. | eassumption ]
+                   | lazymatch goal with
+                     | [ |- Some _ = Some _ ] => fail
+                     | [ |- None = Some _ ] => exfalso; eapply @wf_interp_not_None; [ .. | unfold Syntax.Named.Interp in *; eassumption ]
+                     | [ |- ?x = Some _ ] => destruct x eqn:?; [ apply f_equal | ]
+                     end ] ].
+      move e at bottom.
+      move e1 at bottom.
+      clear dependent e1.
+
+  Admitted.
+End language.
